Refactor DeleteEdges.lean

ErdosStoneSimonovits/Combinatorics/SimpleGraph/DeleteEdges.lean
@@ -20,12 +20,12 @@ end DeleteEdges
 section DeleteIncidenceSet
 
 /-- Given a vertex `x`, remove the edges incident to `x` from the edge set. -/
-abbrev deleteIncidenceSet (G : SimpleGraph V) (x : V) : SimpleGraph V :=
+def deleteIncidenceSet (G : SimpleGraph V) (x : V) : SimpleGraph V :=
   G.deleteEdges (G.incidenceSet x)
 
 lemma deleteIncidenceSet_adj {G : SimpleGraph V} {x v₁ v₂ : V} :
     (G.deleteIncidenceSet x).Adj v₁ v₂ ↔ G.Adj v₁ v₂ ∧ v₁ ≠ x ∧ v₂ ≠ x := by
-  rw [deleteEdges_adj, mk'_mem_incidenceSet_iff]
+  rw [deleteIncidenceSet, deleteEdges_adj, mk'_mem_incidenceSet_iff]
   tauto
 
 lemma deleteIncidenceSet_le (G : SimpleGraph V) (x : V) : G.deleteIncidenceSet x ≤ G :=
@@ -39,18 +39,18 @@ lemma edgeSet_fromEdgeSet_incidenceSet (G : SimpleGraph V) (x : V) :
 /-- The edge set of `G.deleteIncidenceSet x` is the edge set of `G` set difference the incidence
 set of the vertex `x`. -/
 theorem edgeSet_deleteIncidenceSet (G : SimpleGraph V) (x : V) :
-    (G.deleteIncidenceSet x).edgeSet = G.edgeSet \ (G.incidenceSet x) := by
-  simp_rw [deleteEdges, edgeSet_sdiff, edgeSet_fromEdgeSet_incidenceSet]
+    (G.deleteIncidenceSet x).edgeSet = G.edgeSet \ G.incidenceSet x := by
+  simp_rw [deleteIncidenceSet, deleteEdges, edgeSet_sdiff, edgeSet_fromEdgeSet_incidenceSet]
 
 /-- The support of `G.deleteIncidenceSet x` is a subset of the support of `G` set difference the
 singleton set `{x}`. -/
-theorem deleteIncidenceSet_support_subset (G : SimpleGraph V) (x : V) :
+theorem support_deleteIncidenceSet_subset (G : SimpleGraph V) (x : V) :
     (G.deleteIncidenceSet x).support ⊆ G.support \ {x} :=
   fun _ ↦ by simp_rw [mem_support, deleteIncidenceSet_adj]; tauto
 
 /-- If the vertex `x` is not in the set `s`, then the induced subgraph in `G.deleteIncidenceSet x`
 by `s` is equal to the induced subgraph in `G` by `s`. -/
-theorem deleteIncidenceSet_induce_of_not_mem (G : SimpleGraph V) {s : Set V} {x : V} (h : x ∉ s) :
+theorem induce_deleteIncidenceSet_of_not_mem (G : SimpleGraph V) {s : Set V} {x : V} (h : x ∉ s) :
     (G.deleteIncidenceSet x).induce s = G.induce s := by
   ext v₁ v₂
   simp_rw [comap_adj, Function.Embedding.coe_subtype, deleteIncidenceSet_adj, and_iff_left_iff_imp]
@@ -58,30 +58,34 @@ theorem deleteIncidenceSet_induce_of_not_mem (G : SimpleGraph V) {s : Set V} {x 
 
 variable [Fintype V] [DecidableEq V]
 
+instance {G : SimpleGraph V} [DecidableRel G.Adj] {x : V} :
+    DecidableRel (G.deleteIncidenceSet x).Adj :=
+  inferInstanceAs <| DecidableRel (G.deleteEdges (G.incidenceSet x)).Adj
+
 /-- Deleting the incidence set of the vertex `x` retains the same number of edges as in the induced
 subgraph of the vertices `{x}ᶜ`. -/
 theorem card_edgeFinset_induce_compl_singleton (G : SimpleGraph V) [DecidableRel G.Adj] (x : V) :
     #(G.induce {x}ᶜ).edgeFinset = #(G.deleteIncidenceSet x).edgeFinset := by
   have h_not_mem : x ∉ ({x}ᶜ : Set V) := Set.not_mem_compl_iff.mpr (Set.mem_singleton x)
   simp_rw [Set.toFinset_card,
-    ← G.deleteIncidenceSet_induce_of_not_mem h_not_mem, ← Set.toFinset_card]
+    ← G.induce_deleteIncidenceSet_of_not_mem h_not_mem, ← Set.toFinset_card]
   apply card_edgeFinset_induce_of_support_subset
   trans G.support \ {x}
-  · exact deleteIncidenceSet_support_subset G x
+  · exact support_deleteIncidenceSet_subset G x
   · rw [Set.compl_eq_univ_diff]
     exact Set.diff_subset_diff_left (Set.subset_univ G.support)
 
 /-- The finite edge set of `G.deleteIncidenceSet x` is the finite edge set of the simple graph `G`
 set difference the finite incidence set of the vertex `x`. -/
 theorem edgeFinset_deleteIncidenceSet_eq_sdiff (G : SimpleGraph V) [DecidableRel G.Adj] (x : V) :
-    (G.deleteIncidenceSet x).edgeFinset = G.edgeFinset \ (G.incidenceFinset x) := by
+    (G.deleteIncidenceSet x).edgeFinset = G.edgeFinset \ G.incidenceFinset x := by
   rw [incidenceFinset, ← Set.toFinset_diff, Set.toFinset_inj]
   exact G.edgeSet_deleteIncidenceSet x
 
 /-- Deleting the incident set of the vertex `x` deletes exactly `G.degree x` edges from the edge
 set of the simple graph `G`. -/
 theorem card_edgeFinset_deleteIncidenceSet (G : SimpleGraph V) [DecidableRel G.Adj] (x : V) :
-    #(G.deleteIncidenceSet x).edgeFinset = #G.edgeFinset-G.degree x := by
+    #(G.deleteIncidenceSet x).edgeFinset = #G.edgeFinset - G.degree x := by
   simp_rw [← card_incidenceFinset_eq_degree, ← card_sdiff (G.incidenceFinset_subset x),
     edgeFinset_deleteIncidenceSet_eq_sdiff]
 
@@ -92,7 +96,8 @@ theorem edgeFinset_deleteIncidenceSet_eq_filter (G : SimpleGraph V) [DecidableRe
   rw [edgeFinset_deleteIncidenceSet_eq_sdiff, sdiff_eq_filter]
   apply filter_congr
   intro _ h
-  rw [incidenceFinset, Set.mem_toFinset, incidenceSet, Set.mem_setOf_eq, not_and, Classical.imp_iff_right_iff]
+  rw [incidenceFinset, Set.mem_toFinset, incidenceSet,
+    Set.mem_setOf_eq, not_and, Classical.imp_iff_right_iff]
   left
   rwa [mem_edgeFinset] at h
 
@@ -105,7 +110,7 @@ theorem card_support_deleteIncidenceSet
   simp_rw [← Set.card_singleton x, ← Set.toFinset_card, ← card_sdiff hx, ← Set.toFinset_diff]
   apply card_le_card
   rw [Set.toFinset_subset_toFinset]
-  exact G.deleteIncidenceSet_support_subset x
+  exact G.support_deleteIncidenceSet_subset x
 
 end DeleteIncidenceSet
 
